src/program_proof/rsm/pure/word.v
@@ -1,12 +1,16 @@
 From iris.proofmode Require Import proofmode.
 From Perennial.Helpers Require Import Integers.
 
-Lemma uint_nat_W64 (n : nat) :
+Lemma uint_nat_W64_0 :
+  uint.nat (W64 0) = O.
+Proof. word. Qed.
+
+Lemma uint_nat_W64_of_nat (n : nat) :
   n < 2 ^ 64 ->
   uint.nat (W64 n) = n.
 Proof. intros H. word. Qed.
 
 Lemma uint_nat_word_add_S (x : u64) :
   uint.Z x < 2 ^ 64 - 1 ->
-  (uint.nat (w64_word_instance.(word.add) x (W64 1))) = S (uint.nat x).
+  (uint.nat (word.add x (W64 1))) = S (uint.nat x).
 Proof. intros H. word. Qed.
